wip

theories/sessiontypes2.v
@@ -1,4 +1,7 @@
 From iris.proofmode Require Import base tactics classes.
+From diris Require Import util.
+Ltac inv a := inversion a; simplify_eq.
+Ltac invc a := inv a; clear a.
 
 Definition chan := nat.
 
@@ -18,7 +21,7 @@ Inductive val :=
     | Nat : nat -> val
     | Pair : val -> val -> val
     | Fun : string -> expr -> val
-    | Chan : endpoint-> val
+    | Chan : endpoint -> val
 
 with expr :=
     | Val : val -> expr
@@ -58,6 +61,22 @@ Fixpoint dual ct :=
     end.
 
 Definition heapT := gmap endpoint chan_type.
+
+(* Definition jProp := heapT -> Prop.
+
+Definition jWand (p q : jProp) : jProp :=
+    λ Σ, ∀ Σ', Σ ##ₘ Σ' -> p Σ' -> q (Σ ∪ Σ').
+
+Definition jEntails (p q : jProp) : Prop :=
+  ∀ Σ', p Σ' -> q Σ'.
+
+Inductive val_typed : val -> type -> jProp :=
+    | Unit_typed :
+        val_typed Unit UnitT ∅
+    | Pair_typed : ∀ a b aT bT,
+        jEntails (val_typed a aT) $
+        jWand (val_typed b bT) $
+              (val_typed (Pair a b) (PairT aT bT)). *)
 
 Inductive val_typed : heapT -> val -> type -> Prop :=
     | Unit_typed :
@@ -203,9 +222,9 @@ Lemma subst_typed Σv Σe Γ e eT v vT x :
   typed (Σv ∪ Σe) (delete x Γ) (subst x v e) eT.
 Proof.
   intros DΣ DΓ Hv Ht. induction Ht; simpl.
-  - apply lookup_empty_Some in DΓ as [].
-  - apply lookup_singleton_Some in DΓ as [-> ->].
-    rewrite delete_singleton. rewrite decide_True; eauto.
+  - simplify_map_eq.
+  - simplify_map_eq.
+    rewrite delete_singleton.
     rewrite right_id. by constructor.
   - apply lookup_union_Some' in DΓ as [[]|[]]; last done.
     + erewrite (typed_no_var_subst e2); eauto.
@@ -336,38 +355,40 @@ Definition set_send (h : heap) (c : endpoint) (buf : list val) : heap :=
   | None => h
   end.
 
-Inductive head_step : expr -> heap -> expr -> heap -> Prop :=
-    | App_head_step : ∀ x e h a,
-        head_step (App (Val (Fun x e)) (Val a)) h (subst x a e) h
-    | Lam_head_step : ∀ x e h,
-        head_step (Lam x e) h (Val (Fun x e)) h
-    | Send_head_step : ∀ h c y buf,
-        lookup_send h c = Some buf ->
-        head_step (Send (Val (Chan c)) (Val y)) h (Val (Chan c)) (set_recv h c (buf ++ [y]))
-    | Recv_head_step : ∀ h c y buf,
-        lookup_recv h c = Some (y::buf) ->
-        head_step (Recv (Val (Chan c))) h (Val (Pair (Chan c) y)) (set_send h c buf)
-    | If_head_step1 : ∀ n h e1 e2,
+Inductive pure_step : expr -> expr -> Prop :=
+    | App_step : ∀ x e a,
+        pure_step (App (Val (Fun x e)) (Val a)) (subst x a e)
+    | Lam_step : ∀ x e,
+        pure_step (Lam x e) (Val (Fun x e))
+    | If_step1 : ∀ n e1 e2,
         n ≠ 0 ->
-        head_step (If (Val (Nat n)) e1 e2) h e1 h
-    | If_head_step2 : ∀ h e1 e2,
-        head_step (If (Val (Nat 0)) e1 e2) h e2 h
-    | Let_head_step : ∀ x v e h,
-        head_step (Let x (Val v) e) h (subst x v e) h
-    | LetUnit_head_step : ∀ e h,
-        head_step (LetUnit (Val Unit) e) h e h
-    | LetProd_head_step : ∀ x1 x2 v1 v2 e h,
-        head_step (LetProd x1 x2 (Val (Pair v1 v2)) e) h (subst x1 v1 $ subst x2 v2 e) h
+        pure_step (If (Val (Nat n)) e1 e2) e1
+    | If_step2 : ∀ e1 e2,
+        pure_step (If (Val (Nat 0)) e1 e2) e2
+    | Let_step : ∀ x v e,
+        pure_step (Let x (Val v) e) (subst x v e)
+    | LetUnit_step : ∀ e,
+        pure_step (LetUnit (Val Unit) e) e
+    | LetProd_step : ∀ x1 x2 v1 v2 e,
+        pure_step (LetProd x1 x2 (Val (Pair v1 v2)) e) (subst x1 v1 $ subst x2 v2 e).
+
+Inductive head_step : expr -> heap -> expr -> heap -> list expr -> Prop :=
+    | Pure_step : ∀ e e' h,
+        pure_step e e' -> head_step e h e' h []
+    | Send_step : ∀ h c y buf,
+        lookup_send h c = Some buf ->
+        head_step (Send (Val (Chan c)) (Val y)) h (Val (Chan c)) (set_recv h c (buf ++ [y])) []
+    | Recv_step : ∀ h c y buf,
+        lookup_recv h c = Some (y::buf) ->
+        head_step (Recv (Val (Chan c))) h (Val (Pair (Chan c) y)) (set_send h c buf) []
     | Close_step : ∀ c h,
         lookup_recv h c = Some [] ->
-        head_step (Close (Val (Chan c))) h (Val Unit) h.
-
-Lemma head_step_deterministic e s e1 e2 s1 s2 :
-    head_step e s e1 s1 -> head_step e s e2 s2 -> e1 = e2 ∧ s1 = s2.
-Proof.
-    intros H1 H2.
-    induction H1; inversion H2; simplify_eq; eauto.
-Qed.
+        head_step (Close (Val (Chan c))) h (Val Unit) h []
+    | Fork_step : ∀ v (h : heap),
+        head_step
+          (Fork (Val v)) h
+          (Val $ Chan (length h, true)) (h++[([],[])])
+          [App (Val v) (Val (Chan (length h, false)))].
 
 Inductive ctx1 : (expr -> expr) -> Prop :=
     | Ctx_App_l : ∀ e, ctx1 (λ x, App x e)
@@ -384,7 +405,33 @@ Inductive ctx1 : (expr -> expr) -> Prop :=
 
 Inductive ctx : (expr -> expr) -> Prop :=
     | Ctx_nil : ctx (λ x, x)
-    | Ctx_cons : ∀ k1 k2, ctx1 k1 -> ctx k2 -> ctx (k1 ∘ k2).
+    | Ctx_cons : ∀ k1 k2, ctx1 k1 -> ctx k2 -> ctx (λ x, (k1 (k2 x))).
+
+Inductive ctx_step : expr -> heap -> expr -> heap -> list expr -> Prop :=
+  | Ctx_step : ∀ k e h e' h' ts,
+      ctx k -> head_step e h e' h' ts -> ctx_step (k e) h (k e') h' ts.
+
+Inductive step : list expr -> heap -> list expr -> heap -> Prop :=
+  | Head_step : ∀ e e' h h' i ts es,
+      ctx_step e h e' h' ts ->
+      es !! i = Some e ->
+      step es h (<[i := e']> es ++ ts) h'.
+
+(* Closure of the step relation; this is used in the theorem statement. *)
+Inductive steps : list expr -> heap -> list expr -> heap -> Prop :=
+  | Trans_step : ∀ e1 e2 e3 s1 s2 s3,
+      step e1 s1 e2 s2 ->
+      steps e2 s2 e3 s3 ->
+      steps e1 s1 e3 s3
+  | Empty_step : ∀ e1 s1,
+      steps e1 s1 e1 s1.
+
+(* Lemma foo :
+  ctx k ->
+  typed (Σk ∪ Σ1) (k e1) A ->
+  typed Σ1 e1 B ->
+  typed Σ2 e2 B ->
+  typed (Σk ∪ Σ2) (k e2) A. *)
 
 Lemma ctx_app k1 k2 : ctx k1 -> ctx k2 -> ctx (k1 ∘ k2).
 Proof.
@@ -392,128 +439,359 @@ Proof.
   apply (Ctx_cons k1); eauto.
 Qed.
 
-Lemma ctx1_headstep_val k e s e' s' : ctx1 k -> head_step (k e) s e' s' -> ∃ v, e = Val v.
+Lemma ctx1_headstep_val k e s e' s' : ctx1 k -> head_step (k e) s e' s' [] -> ∃ v, e = Val v.
 Proof.
-    intros H. inversion H; intro; inversion H1; simplify_eq; eauto.
+    intros H. inversion H; intro; inversion H1; inv H2; eauto.
 Qed.
 
 Lemma ctx_not_val k e v : ctx k -> k e = Val v -> k = (λ x, x) ∧ e = Val v.
 Proof.
   induction 1; eauto; simpl. intro.
-  inversion H; simplify_eq.
+  inv H.
 Qed.
 
-Ltac cnv := match goal with
-  | [C : ctx ?k, H : ?k _ = Val _ |- _] => apply ctx_not_val in H as (-> & ->); eauto
-  | [C : ctx ?k, H : Val _ = ?k _ |- _] => symmetry in H; apply ctx_not_val in H as (-> & ->); eauto
-  end; match goal with
-  [H : head_step (Val _) _ _ _ |- _] => inversion H
-  end.
-
-Lemma ctx_headstep k1 e1 k2 e2 s : ctx k1 -> ctx k2 ->
-  k1 e1 = k2 e2 -> (∃ e1' s', head_step e1 s e1' s') -> (∃ e2' s', head_step e2 s e2' s') ->
-  k1 = k2 ∧ e1 = e2.
+Lemma pure_step_typed e e' Σ A :
+  pure_step e e' ->
+  typed Σ ∅ e A ->
+  typed Σ ∅ e' A.
 Proof.
-  intros C1.
-  revert k2.
-  induction C1 as [|C1' k1']; intros k2 C2 Heq.
-  - induction C2; eauto.
-    intros (e1' & s1 & Hs1) (e2' & s2 & Hs2).
-    inversion H; simplify_eq; simpl in *; inversion Hs1; simplify_eq; cnv.
-  - induction C2.
-    + intros (e1' & s1 & Hs1) (e2' & s2 & Hs2).
-      inversion H; simplify_eq; simpl in *; inversion Hs2; simplify_eq; cnv.
-    + inversion H; inversion H0; simplify_eq;
-      try (intros; assert (k1' = k2 ∧ e1 = e2) as (-> & ->); eauto);
-      destruct H1 as (e1' & s1' & Hs1); destruct H2 as (e2' & s2' & Hs2); try cnv.
+  intros Hps Hty.
+  destruct Hps.
+  + invc Hty. rewrite H.
+    invc H7.
+    invc H5.
+    invc H7.
+    replace (∅ : envT) with (delete x {[x := t1]} : envT) by
+      (by rewrite delete_singleton).
+    rewrite map_union_comm; eauto.
+    eapply subst_typed; eauto.
+    eapply lookup_singleton.
+  + invc Hty.
+    econstructor. econstructor. rewrite left_id in H5. done.
+  + inv Hty. rewrite H0.
+    inv H7.
+    inv H5. rewrite left_id.
+    rewrite left_id in H0. rewrite H0 in H9. done.
+  + inv Hty. rewrite H.
+    inv H6.
+    inv H4. rewrite left_id.
+    rewrite left_id in H. rewrite H in H9. done.
+  + inv Hty. rewrite H.
+    inv H8. rewrite left_id in H. simplify_eq.
+    rewrite left_id in H9.
+    replace (∅ : envT) with (delete x {[x := t1]} : envT) by
+      (by rewrite delete_singleton).
+    eapply subst_typed; eauto.
+    eapply lookup_singleton.
+  + inv Hty. inv H5.
+    rewrite left_id in H. simplify_eq. rewrite left_id.
+    inv H6. rewrite left_id. done.
+  + inv Hty. rewrite H.
+    inv H11.
+    inv H3.
+    rewrite left_id in H. simplify_eq.
+    rewrite left_id in H12.
+    replace (∅) with (delete x1 (delete x2 ({[x1 := t11]} ∪ {[x2 := t12]})) : envT).
+    2: { rewrite delete_union delete_singleton right_id delete_singleton_ne; eauto.
+          rewrite delete_singleton. done. }
+    rewrite <-(assoc union).
+    eapply subst_typed; eauto.
+    * solve_map_disjoint.
+    * rewrite delete_union delete_singleton right_id delete_singleton_ne; eauto.
+      apply lookup_singleton.
+    * eapply subst_typed; eauto. solve_map_disjoint.
+      apply lookup_union_Some_r.
+      {
+        rewrite map_disjoint_alt. intro.
+        destruct (decide (i = x1)) as [->|?].
+        - right. apply lookup_singleton_ne; eauto.
+        - left. apply lookup_singleton_ne; eauto.
+      }
+      apply lookup_singleton.
 Qed.
 
-Inductive ctx_step : expr -> heap -> expr -> heap -> Prop :=
-    | Ctx_step : ∀ k e1 e2 s1 s2,
-        ctx k -> head_step e1 s1 e2 s2 -> ctx_step (k e1) s1 (k e2) s2.
+Definition ctx_typed (Σ : heapT) (Γ : envT) (k : expr -> expr) (A : type) (B : type) :=
+    ∀ e Σ' Γ', Σ ##ₘ Σ' -> Γ ##ₘ Γ' -> typed Σ' Γ' e A -> typed (Σ ∪ Σ') (Γ ∪ Γ') (k e) B.
 
-Lemma ctx_step_deterministic e s e1 e2 s1 s2 :
-    ctx_step e s e1 s1 -> ctx_step e s e2 s2 -> e1 = e2 ∧ s1 = s2.
+Lemma ctx_typed_typed Σ Σ' k A B Γ Γ' e :
+  Σ ##ₘ Σ' -> Γ ##ₘ Γ' -> ctx_typed Σ Γ k A B -> typed Σ' Γ' e A -> typed (Σ ∪ Σ') (Γ ∪ Γ') (k e) B.
 Proof.
-    intros H1 H2. inversion H1. inversion H2. simplify_eq.
-    assert (k = k0 ∧ e0 = e4) as (-> & ->) by (eapply ctx_headstep; eauto).
-    assert (e3 = e5 ∧ s1 = s2) as (-> & ->) by (eapply head_step_deterministic; eauto); eauto.
+  unfold ctx_typed; eauto.
 Qed.
 
-(* TODO: make this a relation on pairs, then steps = rtc step *)
-(* We put the fork step here because it needs to spawn a new thread. *)
-Inductive step : list expr -> heap -> list expr -> heap -> Prop :=
-    | Head_step : ∀ e1 e2 s1 s2 es i k,
-        ctx k ->
-        head_step e1 s1 e2 s2 ->
-        es !! i = Some (k e1) ->
-        step es s1 (<[i := (k e2)]> es) s2
-    | Fork_step : ∀ (es : list expr) i v (h : heap) k,
-        let l := length h in
-        ctx k ->
-        es !! i = Some (k $ Fork (Val v)) ->
-        step es h
-            (<[i := k $ Val (Chan (l,true))]> es ++ [App (Val v) (Val (Chan (l,false)))])
-            (h++[([],[])]).
+Lemma ctx_typed_compose Σ Σ' Γ Γ' k k' A B C :
+  Σ' ##ₘ Σ -> Γ' ##ₘ Γ -> ctx_typed Σ Γ k A B -> ctx_typed Σ' Γ' k' B C -> ctx_typed (Σ' ∪ Σ) (Γ' ∪ Γ) (k' ∘ k) A C.
+Proof.
+  intros Hdisj Hdisj' Hct1 Hct2.
+  unfold ctx_typed in *.
+  intros e Σ1 Γ1 Hdisj1 Hdisj1' Htyped1. simpl.
+  rewrite <-!(assoc union).
+  solve_map_disjoint.
+Qed.
 
-(* Closure of the step relation; this is used in the theorem statement. *)
-Inductive steps : list expr -> heap -> list expr -> heap -> Prop :=
-    | Trans_step : ∀ e1 e2 e3 s1 s2 s3,
-        step e1 s1 e2 s2 ->
-        steps e2 s2 e3 s3 ->
-        steps e1 s1 e3 s3
-    | Empty_step : ∀ e1 s1,
-        steps e1 s1 e1 s1.
+Lemma typed_ctx1_typed Σ Γ B k e :
+  ctx1 k -> typed Σ Γ (k e) B ->
+  ∃ Σ1 Σ2 Γ1 Γ2 A,
+    Σ = Σ1 ∪ Σ2 ∧ Σ1 ##ₘ Σ2 ∧
+    Γ = Γ1 ∪ Γ2 ∧ Γ1 ##ₘ Γ2 ∧
+    ctx_typed Σ2 Γ2 k A B ∧ typed Σ1 Γ1 e A.
+Proof.
+  intros Hctx1 Htyped.
+  destruct Hctx1; invc Htyped;
+  try solve [
+    do 5 eexists;
+    split; last split; last split; last split; last split; eauto;
+    intros e' Σ' Γ' Hdisj1 Hdisj2 Htyped';
+    rewrite (map_union_comm Σ2); eauto;
+    rewrite (map_union_comm Γ2); eauto;
+    econstructor; try solve_map_disjoint; eauto
+  ]; try solve [
+    do 5 eexists;
+    split; last split; last split; last split; last split; last eauto; eauto using map_union_comm;
+    [by apply map_union_comm|by apply map_union_comm|];
+    intros e' Σ' Γ' Hdisj1 Hdisj2 Htyped';
+    econstructor; try solve_map_disjoint; eauto
+  ]; solve [
+    exists Σ; exists ∅; exists Γ; exists ∅; eexists;
+    split; last split; last split; last split; last split; last eauto; try rewrite right_id; eauto;
+    try apply map_disjoint_empty_r;
+    intros e' Σ' Γ' Hdisj1 Hdisj2 Htyped';
+    rewrite !left_id;
+    econstructor; try solve_map_disjoint; eauto
+  ].
+Qed.
 
-Inductive all_values : list expr -> Prop :=
-    | AV_nil : all_values []
-    | AV_cons : ∀ es v, all_values es -> all_values (Val v :: es).
-    (* TODO: add case for waiting on Recv on an empty buffer for now *)
+Lemma typed_ctx_typed Σ Γ B k e :
+  ctx k -> typed Σ Γ (k e) B ->
+  ∃ Σ1 Σ2 Γ1 Γ2 A,
+    Σ = Σ1 ∪ Σ2 ∧ Σ1 ##ₘ Σ2 ∧
+    Γ = Γ1 ∪ Γ2 ∧ Γ1 ##ₘ Γ2 ∧
+    ctx_typed Σ1 Γ1 k A B ∧ typed Σ2 Γ2 e A.
+Proof.
+  intros Hctx. revert Σ Γ B. induction Hctx; intros Σ Γ B Htyped.
+  - exists ∅, Σ.
+    exists ∅, Γ, B.
+    rewrite !left_id. repeat split; try apply map_disjoint_empty_l; eauto.
+    unfold ctx_typed. intros e' Σ' Γ' _ _. rewrite !left_id. eauto.
+  - simpl in *.
+    eapply typed_ctx1_typed in Htyped; eauto.
+    destruct Htyped as (Σ1 & Σ2 & Γ1 & Γ2 & A & Heq1 & Hdisj1 &
+      Heq2 & Hdisj2 & Hctx_typed & Htyped). subst.
+    eapply IHHctx in Htyped.
+    destruct Htyped as (Σ11 & Σ12 & Γ11 & Γ12 & A' & Heq1' & Hdisj1' &
+      Heq2' & Hdisj2' & Hctx_typed' & Htyped). subst.
+    exists (Σ2 ∪ Σ11),Σ12.
+    exists (Γ2 ∪ Γ11),Γ12.
+    eexists.
+    repeat split; try solve_map_disjoint; eauto.
+    + rewrite map_union_comm; eauto. by rewrite assoc.
+    + rewrite map_union_comm; eauto. by rewrite assoc.
+    + eapply ctx_typed_compose; eauto; solve_map_disjoint.
+Qed.
 
-(* TODO: rethink bufs_typed and the invariant *)
+Lemma map_positive {V} `{Countable K} (A B : gmap K V) :
+  A ∪ B = ∅ -> A = ∅ ∧ B = ∅.
+Proof.
+  intros. apply map_positive_l in H0 as H0'. subst. rewrite left_id in H0. done.
+Qed.
 
-Definition disjoint (xs : list heapT) :=
-    forall i j h1 h2, i ≠ j ->
-        xs !! i = Some h1 -> xs !! j = Some h2 -> h1 ##ₘ h2.
 
-Inductive bufs_typed : heapT * list val * chan_type -> heapT * list val * chan_type -> Prop :=
-  | BT_emp : ∀ ct, bufs_typed (∅, [], ct) (∅, [], dual ct)
+Inductive bufs_typed : heapT -> list val * chan_type -> list val * chan_type -> Prop :=
+  | BT_emp : ∀ ct, bufs_typed ∅ ([], ct) ([], dual ct)
   | BT_consL : ∀ Σ1 Σ2 v vT vs ct c,
     Σ1 ##ₘ Σ2 ->
     val_typed Σ1 v vT ->
-    bufs_typed (Σ2, vs, ct) (∅, [], c) ->
-    bufs_typed (Σ1 ∪ Σ2, v::vs, ct) (∅, [], RecvT vT c)
+    bufs_typed Σ2 (vs, ct) ([], c) ->
+    bufs_typed (Σ1 ∪ Σ2) (v::vs, ct) ([], RecvT vT c)
   | BT_consR : ∀ Σ1 Σ2 v vT vs ct c,
     Σ1 ##ₘ Σ2 ->
     val_typed Σ1 v vT ->
-    bufs_typed (∅, [], c) (Σ2, vs, ct) ->
-    bufs_typed (∅, [], RecvT vT c) (Σ1 ∪ Σ2, v::vs, ct).
+    bufs_typed Σ2 ([], c) (vs, ct) ->
+    bufs_typed (Σ1 ∪ Σ2) ([], RecvT vT c) (v::vs, ct).
 
-Definition invariant (es : list expr) (h : heap) : Prop :=
-  ∃ (Σ : heapT) (Σs : list heapT) (Σh1 Σh2 : list heapT),
-    disjoint_union Σ (Σh1 ++ Σh2 ++ Σs) ∧
-    Forall2 (λ Σ e, typed Σ ∅ e UnitT) Σs es ∧
-    length Σh1 = length h ∧
-    length Σh2 = length h ∧
-    ∀ l b ct, Σ !! (l,b) = Some ct ->
-      ∃ b1 b2 ct' Σ1 Σ2,
-        Σ !! (l,negb b) = Some ct' ∧
-        lookup_recv h (l,b) = Some b1 ∧
-        lookup_recv h (l,negb b) = Some b2 ∧
-        Σh1 !! l = Some Σ1 ∧
-        Σh2 !! l = Some Σ2 ∧
-        bufs_typed (Σ1, b1, ct) (Σ2, b2, ct').
+Definition none_to_end (ct' : option chan_type) : chan_type :=
+  match ct' with
+  | None => EndT
+  | Some ct => ct
+  end.
+
+Definition invariant (threads : list expr) (chans : heap) : Prop :=
+  ∃ (threadΣs : list heapT) (chanΣs : list heapT),
+    disjoint (threadΣs ++ chanΣs) ∧
+    Forall2 (λ Σt t, typed Σt ∅ t UnitT) threadΣs threads ∧
+    let Σ := ⋃ (threadΣs ++ chanΣs) in
+    Forall3 (λ (Σbuf : heapT) '(buf1,buf2) (i : nat),
+        bufs_typed Σbuf
+            (buf1, none_to_end (Σ !! (i,true)))
+            (buf2, none_to_end (Σ !! (i,false)))
+      ) chanΣs chans (seq 0 (length chans)).
+
+Lemma preservation es h es' h' :
+  invariant es h -> step es h es' h' -> invariant es' h'.
+Proof.
+  intros Hinv Hstep.
+  destruct Hstep.
+  destruct H.
+  unfold invariant in *.
+  destruct Hinv as (threadΣs & chanΣs & Hdisj & Hthreads & Hheap).
+  destruct (Forall2_lookup_r _ _ _ _ _ Hthreads H0) as (Σ' & Hsome & Htyped).
+  eapply typed_ctx_typed in Htyped; eauto.
+  destruct Htyped as (Σ1 & Σ2 & Γ1 & Γ2 & A & Heq1 & Hdisj1 & Heq2 & Hdisj2 & Hctx_typed & Htyped).
+  symmetry in Heq2. apply map_positive in Heq2 as [-> ->]. clear Hdisj2. subst.
+
+  destruct H1; try rewrite right_id.
+  - eapply pure_step_typed in H1; eauto.
+    eapply ctx_typed_typed in H1; eauto; last solve_map_disjoint.
+    rewrite left_id in H1.
+    exists threadΣs, chanΣs.
+    split; first done. split; last done.
+    replace threadΣs with (<[ i := (Σ1 ∪ Σ2) ]> threadΣs : list heapT) by
+      (by eapply list_insert_id in Hsome).
+    apply Forall2_insert; done.
+  - invc Htyped.
+    apply map_positive in H2 as [-> ->]. clear H7.
+    invc H10.
+    invc H8.
+    invc H6.
+    (* Need to get our hands on the bufs typed here *)
+    (* Need to get the exists right here, then the rest should be easier *)
+    admit.
+  - invc Htyped.
+    invc H5.
+    invc H4.
+    admit.
+  - invc Htyped.
+    invc H5.
+    invc H4.
+    exists (<[ i := Σ1 ]> threadΣs), chanΣs.
+    split.
+    {
+      SearchAbout insert app.
+      apply disjoint_update.
+      (* Need lemma about disjoint here *)
+      admit.
+    }
+    split.
+    {
+      apply Forall2_insert; first done.
+      assert (typed ∅ ∅ (Val Unit) UnitT) by (econstructor; econstructor).
+      eapply ctx_typed_typed in H2; last done; rewrite ?right_id in H2; solve_map_disjoint.
+    }
+    {
+      eapply Forall3_impl; first done.
+      intros Σh [buf1 buf2] j Hbt.
+      (* Need lemma about lookup in foldr union *)
+      admit.
+    }
+  - invc Htyped.
+    set c := length h.
+    exists (<[ i := Σ1 ∪ {[ (c,true) := ct ]} ]> threadΣs ++ [Σ2 ∪ {[ (c,false) := dual ct ]}]).
+    exists (chanΣs ++ [∅]).
+    split.
+    {
+      admit.
+    }
+    split.
+    {
+      admit.
+    }
+    {
+      admit.
+    }
+Admitted.
+
+Inductive final : expr -> Prop :=
+  | final_val : ∀ v, final (Val v)
+  | final_recv : ∀ c k, ctx k -> final (k $ Recv $ Val $ Chan c).
+
+Lemma ctx_step_cons k e h e' h' ts :
+  ctx1 k -> ctx_step e h e' h' ts -> ctx_step (k e) h (k e') h' ts.
+Proof.
+  intros Hctx1 Hcs.
+  destruct Hcs.
+  eapply (Ctx_step (λ x, k (k0 x))).
+  - constructor; done.
+  - done.
+Qed.
+
+Lemma progress1 Σ e h A :
+  typed Σ ∅ e A -> final e ∨ ∃ e' h' ts, ctx_step e h e' h' ts.
+Proof.
+  intros Htyped.
+  revert A Σ Htyped; induction e; intros A Σ Htyped.
+  - left. constructor.
+  - exfalso. admit.
+  - invc Htyped.
+    apply map_positive in H as [-> ->]. clear H4.
+    edestruct IHe1; first done.
+    + invc H;[|invc H5].
+      invc H5.
+      edestruct IHe2; first done.
+      * invc H.
+        {
+          invc H7.
+          invc H1.
+          right.
+          do 3 eexists.
+          eapply (Ctx_step id). constructor.
+          constructor. constructor.
+        }
+        {
+          invc H7.
+          admit.
+        }
+      * destruct H as (e'' & h'' & ts & Hcs).
+        invc Hcs. do 3 eexists.
+        eapply (ctx_step_cons (λ x, App (Val v) x)). constructor.
+        constructor. done.
+        done.
+    + destruct H as (e' & h' & ts & Hcs).
+      right. do 3 eexists.
+      eapply (ctx_step_cons (λ x, App x e2)); [constructor|done].
+  - admit.
+  - admit.
+  - admit.
+  - admit.
+  - admit.
+  - admit.
+  - admit.
+  - admit.
+  - admit.
+  - admit.
+  - admit.
+  - admit.
+  - admit.
+Admitted.
+
+Lemma progress es h :
+  invariant es h -> Forall final es ∨ ∃ es' h', step es h es' h'.
+Proof.
+Admitted.
+
+Lemma lookup_one_Some {A} (x : A) i v :
+  [x] !! i = Some v -> x = v ∧ i = 0.
+Proof.
+  destruct i; simpl in *.
+  - intro. simplify_eq. done.
+  - destruct i; simpl; intro; simplify_eq.
+Qed.
+
+Lemma disjoint_singleton (x : heapT) :
+  disjoint [x].
+Proof.
+  unfold disjoint. intros.
+  apply lookup_one_Some in H0 as [_ ->].
+  apply lookup_one_Some in H1 as [_ ->].
+  done.
+Qed.
 
 Theorem invariant_init e : typed ∅ ∅ e UnitT -> invariant [e] [].
 Proof.
-  intros Ht.
+  intros Htyped.
   unfold invariant.
-  exists ∅, [∅ : heapT], [], []. simpl. split.
-  - exists ∅. unfold disj_union. split; eauto. split.
-    + apply map_disjoint_empty_l.
-    + by rewrite left_id_L.
-  - repeat (split;eauto). intros.
-    by apply lookup_empty_Some in H.
+  exists [∅], []. simpl.
+  split; first by apply disjoint_singleton.
+  split; eauto. constructor.
 Qed.
 
 Lemma dual_dual c : dual (dual c) = c.
@@ -552,7 +830,7 @@ Lemma bufs_typed_recv_l Σ Σ' aT vs r vs' r' :
       val_typed Σ1 a aT ∧
       bufs_typed (Σ,vs,r) (Σ2,vs',r').
 Proof.
-  intros H. inversion H; simplify_eq. eauto.
+  intros H. inv H. eauto.
 Qed.
 *)
 
@@ -563,7 +841,7 @@ Lemma bufs_typed_recv_l Σ Σ' a aT vs r vs' r' :
       val_typed Σ1 a aT ∧
       bufs_typed (Σ,vs,r) (Σ2,vs',r').
 Proof.
-  intros H. inversion H. simplify_eq. eauto.
+  intros H. inv H. eauto.
 Qed.
 
 Lemma bufs_typed_recv_r Σ Σ' a aT vs r vs' r' :
@@ -573,7 +851,7 @@ Lemma bufs_typed_recv_r Σ Σ' a aT vs r vs' r' :
       val_typed Σ1 a aT ∧
       bufs_typed (Σ2,vs',r') (Σ,vs,r) .
 Proof.
-  intros H. inversion H. simplify_eq. eauto.
+  intros H. inv H. eauto.
 Qed.
 
 Lemma bufs_typed_send_l Σ Σ' Σ1 Σp a aT vs r vs' r' :
@@ -584,12 +862,12 @@ Lemma bufs_typed_send_l Σ Σ' Σ1 Σp a aT vs r vs' r' :
 Proof.
   revert Σ Σ' Σ1 Σp a aT r vs' r'.
   induction vs as [|v1 vr]; intros Σ Σ' Σ1 Σp a aT r vs' r' Hv Hd Hbt; simpl.
-  - inversion Hbt. simplify_eq.
+  - inv Hbt.
     econstructor. 3: econstructor.
     + apply disj_union_empty_r. apply disj_union_sym in Hd.
       apply disj_union_empty_r in Hd. eauto.
     + eauto.
-  - inversion Hbt. simplify_eq.
+  - inv Hbt.
     econstructor; last first. 2: done.
     + eapply IHvr; last done; first done.
       unfold disj_union in *. split; last done.
@@ -698,7 +976,7 @@ Theorem invariant_preserved es es' h h' :
   invariant es h -> step es h es' h' -> invariant es' h'.
 Proof.
   intros Hinv Hstep.
-  inversion Hstep; simplify_eq.
+  inv Hstep.
   - admit.
     (* TODO: think about the right induction hypothesis here, for the induction over the context *)
   - unfold invariant.
