theories/edoardo.v
@@ -1,0 +1,1470 @@
+Require Export Arith String List Omega.
+Export ListNotations.
+Global Generalizable All Variables.
+
+(*
+# Contents
+
+- Inductive data types
+- Proofs and tactics
+- Data types in canonical representation
+
+# Tactics
+
+Below you can find an overview of the basic tactics of Coq. Most of these
+tactics will be discussed in the lecture, but not all. You should carefully read
+them and try to use them in the exercises.
+
+## Tactics for basic logic
+
+- `assumption` : the assumption rule of logic, it finishes goals if the goal
+   appears among the hypotheses.
+
+   ------------ `assumption`
+    H : P |- P
+
+- `intros x` : performs implication or forall introduction.
+
+    H : P |- Q
+   ------------ `intros H`
+    |- P -> Q
+
+    x : A |- Q x
+   ----------------------  `intros x`
+    |- forall x : A, Q x
+
+  Note that intros can be chained, e.g. one can write `intros x y H1 H2`.
+
+- `revert` : performs implication or forall elimination (in a way that is in
+  opposite direction of `intros`).
+
+     |- P -> Q
+    ------------ `revert H`
+     H : P |- Q
+
+     |- forall x : A, P x
+    ---------------------- `revert x` (if `x` does not appear in any hypothesis)
+     x : A |- P x
+
+  This tactic is most commonly used to _generalize the induction hypothesis_,
+  i.e. before an induction proof to make sure that the induction hypothesis is
+  suitably generalized.
+
+  Note that reverts can be chained, e.g. one can write `revert x y H1`.
+
+- `apply` : performs implication or forall elimination.
+
+     |- Pi a1 .. an          |- Pm a1 .. an
+    ---------------------------------------------------------------------------- 'apply H`
+     H : forall x1 .. xn, (P1 x1 .. xn) -> ... -> (Pm x1 .. xn) -> (Q x1 .. xn)
+     |- Q a0 .. an
+
+- `assert` : performs implication elimination.
+
+     |- P    H : P |- Q
+    --------------------  `assert P as H`
+           |- Q
+
+- `specialize` : performs forall elimination.
+
+     H : P a |- Q
+    ------------------------ `specialize (H a)`
+     H : forall x, P x |- Q
+
+  Note that specialize can be chained, e.g. one can write `specialize H a b`
+
+- `split` : performs conjunction introduction.
+
+     |- P1     |- P2
+    ----------------- `split`
+       |- P1 /\ P2
+
+- `left` : performs (left-) disjunction introduction.
+
+     |- P1
+    ------------- `left`
+     |- P1 \/ P2
+
+- `right` : performs (right-) disjunction introduction.
+
+     |- P2
+    ------------- `right`
+     |- P1 \/ P2
+
+- `destruct` performs elimination of inductive types, in particular, it can
+  be used for conjunction and disjunction elimination as follows:
+
+  For conjunction elimination:
+
+     H : P1, H2 : P2 |- Q
+    ---------------------- `destruct H as [H1 H2]`
+     H : P1 /\ P2 |- Q
+
+  For disjunction elimination:
+
+     H : P1 |- Q    H : P2 |- Q
+    ---------------------------- `destruct H as [H1|H2]`
+     H : P1 \/ P2 |- Q
+
+## Computation
+
+- `simpl` : simplifies the goal by computation. For example, given a goal that
+  contains `S x + y` it will turn it into the same goal but with all occurrences
+  of `S x + y` replaces by `S (x + y)`.
+
+  Alternatively, an hypothesis `H` can be simplified by computation by writing
+  `simpl in H`.
+
+- `unfold` : unfold a definition into its body. For example, when having
+
+    Definition foo := bar.
+
+  Then `unfold foo` will replace all occurrences of `foo` in the goal by `bar.
+  As for `simpl`, one can perform the tactic to a hypothesis `H` by writing
+  `unfold foo in H`.
+
+## Equality
+
+- `reflexivity` : proves goals of the shape `x = x`
+
+    ------- reflexivity
+     x = x
+
+- `discriminate` : discharges goals with an hypothesis of the shape
+
+    --------------------------
+     H : c1 ... = c2 ... |- Q
+
+  Where `c1` and `c2` are different constructors (e.g. `true` and `false, or
+  `O` and `S`).
+
+- `injection` : performs injectivity of constructors.
+
+   Given the following goal, where `c` is a constructor of an inductive data
+   type (for example, `S` or `cons`):
+
+      H1 : x0 = y0, .., Hn : xn = yn |- Q
+     ------------------------------------- `injection H as H1 .. Hn`
+      H : c x0 .. xn = c y0 .. yn |- Q
+
+- `rewrite` substitutes all occurrences of an equality.
+
+     H : x = y |- Q y
+    ------------------ `rewrite H`
+     H : x = y |- P x
+
+     H : x = y |- Q x
+    ------------------ `rewrite <-H`
+     H : x = y |- P y
+
+  The rewrite tactic can also be used in hypotheses, e.g. `rewrite H1 in H2`.
+
+- `f_equal` : proves an equality by proving that all arguments of a function
+   are equal.
+
+     |- x0 = y0   ...   |- xn = yn
+    ------------------------------- `f_equal`
+     |- f x0 .. xn = f y0 ... yn
+
+## Inductive data types
+
+- `destruct` : performs a case analysis. For example, given a natural number
+  `n`, one can write `destruct n as [|n']`, which will generate two goals, one
+  for the case `n = O` and one for the case `n = S n'`.
+
+- `induction` : performs induction. For example, given a natural number
+  `n`, one can write `induction n as [|n' IH]`, which will generate two goals,
+  the base case, and the inductive case, in which the induction hypothesis is
+  called `IH`.
+*)
+
+(* # Introduction *)
+(*
+The underlying theory of Coq is based on the Calculus of Inductive Constructions
+(CIC). CIC is a language that can be used as:
+
+- A typed functional programming language
+- A language to represent mathematical statements
+- A language to represent proofs
+
+As we will see during the summer school, by the Curry Howard Correspondence, all
+of the above concepts are in fact unified, because CIC is a
+
+  higher-order dependently typed programming language
+
+In this lecture, we will not go much into the details of the Curry Howard
+Correspondence, but focus more on a practical use of  Coq to formalize
+programming language semantics.
+*)
+
+(* # Inductive types *)
+(*
+An important aspect of Coq is to keep the underlying theory, the CIC, small.
+This is achieved is not building in the standard data types that we see in
+ordinary programming languages, but instead define these data types in terms of
+unified constructs. Specifically, in Coq, these data types (and many more) can
+be defined by means of inductive types. In the first part of this lecture, I
+will give an introduction to inductive types, ans show how these can be used for
+programming and proving.
+
+Mote, all of the inductive types that we will define are also in the Coq
+standard library. In order to not confuse the standard library results with our
+own definitions, we put our own definitions in a module. That way, after we
+close the module, we can use the results from the Coq standard library for
+subsequent lectures.
+*)
+Module lecture.
+
+(* ## Booleans *)
+(*
+Let us start with one of the simplest data types, the Booleans. In Coq, these
+can de defined through the following definition:
+*)
+
+Inductive bool : Type :=
+  | true : bool
+  | false : bool.
+
+(*
+The lines above introduces a new type called `bool` with _constructors_ `false`
+and `true`. Similar to functional programming languages like OCaml and Haskell,
+we can now define operations by pattern matching.
+*)
+
+Definition andb (b1 b2 : bool) : bool :=
+  match b1 with
+  | true => b2
+  | false => false
+  end.
+
+Definition orb (b1 b2 : bool) : bool :=
+  match b1 with
+  | true => true
+  | false => b2
+  end.
+
+(*
+What makes Coq different from ordinary functional programming languages is that
+we can now prove properties about these operations. For example:
+*)
+Lemma andb_true_l : forall b : bool, andb true b = b.
+Proof.
+  intros b. (* introduce the forall quantifier, and name the variable b *)
+  simpl. (* simplify the goal *)
+  reflexivity. (* both side of the equation are equal *)
+Qed.
+
+(*
+Of course, the above property was rather boring, it followed immediately by
+definition of the function `andb`. Proofs like above, are often called _proof by
+computation_. Let us now consider something slightly more interesting, where we
+will see a new proof technique: proof by _case distinction_.
+*)
+
+Lemma andb_true_r : forall b : bool, andb b true = b.
+Proof.
+  intros b.
+  simpl. (* This does not simplify anything, the reason for it is that `andb` is
+  defined by pattern matching on the first argument. *)
+
+  (* We are now going to use a new proof technique: _proof by case distinction_.
+  In this case, since `b` is of type `bool` we know that it is either `true` or
+  `false`. In Coq we can make such a case distinction using the `destruct`
+  tactic. *)
+  destruct b.
+  (* After this, we get two goals: for `true` and for `false. We can use the
+  bullets `-`, `+` and `*` to structure the subproofs for these cases. *)
+  - (* case `b = true` *)
+    simpl.
+    reflexivity.
+  - (* case `b = false` *)
+    simpl.
+    reflexivity.
+Qed.
+
+(*
+Now let us the combination of both proof techniques to prove another result.
+*)
+Lemma andb_comm : forall b1 b2 : bool, andb b1 b2 = andb b2 b1.
+Proof.
+  intros b1 b2.
+  destruct b1.
+  - destruct b2.
+    + simpl.
+      reflexivity.
+    + simpl.
+      reflexivity.
+  - destruct b2.
+    + simpl.
+      reflexivity.
+    + simpl.
+      reflexivity.
+Qed.
+
+(*
+As we see, the above proof is pretty lengthy and contains a lot of repetition.
+We will now carry out the proof in a shorter and more concise manner.
+
+First observe that our proofs is composed of a sequence of _tactics_ (like
+`intros`, `simpl`, `destruct` and `reflexivity`), each of those separated by a
+period.  The period executes the tactic, and produces a number of subgoals (or
+zero, for example when using `reflexivity`, which are then shown to the user.
+
+Apart from periods, tactics in Coq can also be sequenced using the semicolon
+operator:
+
+  tac1; tac2.
+
+The semantics of this kind of sequencing is a bit different than that of
+`tac1. tac2.`: it will apply `tac2` to all subgoals generated by `tac1`, and
+does not explicitly show goals for the intermediate results. Let us see this
+kind of sequencing in action:
+*)
+
+Lemma andb_comm_short_proof : forall b1 b2 : bool, andb b1 b2 = andb b2 b1.
+Proof.
+  intros b1 b2.
+  destruct b1; destruct b2; simpl; reflexivity.
+Qed.
+
+Lemma andb_assoc : forall b1 b2 b3 : bool,
+  andb b1 (andb b2 b3) = andb (andb b1 b2) b3.
+Proof.
+  intros b1 b2 b3.
+  destruct b1; simpl; reflexivity.
+(* Question: why do we not need to perform a case analysis on `b2` or `b3`? *)
+Qed.
+
+(* # Exercise *)
+(*
+Prove the following lemmas, first try to prove them using the period as
+sequencing operator, and then try to optimize the proof to use the semicolon.
+*)
+Lemma andb_false_l : forall b : bool, andb false b = false.
+Proof. Admitted.
+
+Lemma andb_false_r : forall b : bool, andb b false = false.
+Proof. Admitted.
+
+Lemma andb_diag : forall b, andb b b = b.
+Proof. Admitted.
+
+Lemma orb_true_l : forall b : bool, orb true b = true.
+Proof. Admitted.
+
+Lemma orb_true_r : forall b : bool, orb b true = true.
+Proof. Admitted.
+
+Lemma orb_false_l : forall b : bool, orb false b = b.
+Proof. Admitted.
+
+Lemma orb_false_r : forall b : bool, orb b false = b.
+Proof. Admitted.
+
+Lemma orb_diag : forall b, orb b b = b.
+Proof. Admitted.
+
+Lemma orb_comm : forall b1 b2 : bool, orb b1 b2 = orb b2 b1.
+Proof. Admitted.
+
+Lemma orb_assoc : forall b1 b2 b3 : bool,
+  orb b1 (orb b2 b3) = orb (orb b1 b2) b3.
+Proof. Admitted.
+
+Lemma orb_andb_distr : forall b1 b2 b3,
+  andb b1 (orb b2 b3) = orb (andb b1 b2) (andb b1 b3).
+Proof. Admitted.
+
+(*
+So far we have seen two proof techniques: proof by computation (using the
+`simpl` tactic) and proof by case distinction (using the `destruct` tactic).
+We will now see a new technique: _proof by contradiction_. Before doing that,
+let us take  a look at the way logical negation is defined in Coq:
+
+  ~P := P -> False
+
+So, as we see here, in order to prove `~P`, we have to prove that under the
+assumption of `P` we can prove `False`, i.e. under the assumption of `P`, we
+can prove _anything_.
+*)
+
+Lemma true_neq_false : true <> false.
+Proof.
+  unfold not. (* unfold the definition of negation, which is called `not`, using
+  the `unfold` tactic. *)
+
+  intros H. (* introduce the assumption `H : true = false`. *)
+
+  (* But what to do next? So far we have only proved equalities, but now we have
+  a contradicting equality as an assumption. The reason that this assumption is
+  contradictory is that both sides of the equality involve different
+  constructors. If we end up in such a situation, we can use the `discriminate`
+  tactic to prove anything (include `False`). *)
+  discriminate.
+Qed.
+
+Lemma andb_true_inv : forall b1 b2,
+  andb b1 b2 = true -> b1 = true /\ b2 = true.
+Proof.
+  intros b1 b2 H.
+  (* Since `andb` is defined by pattern matching on the first argument, we
+  perform a case analysis on `b1`. *)
+  destruct b1.
+  - (* case `b1 = true` *)
+    simpl in H. (* The `simpl` tactic can also be used to simplify hypotheses.
+    We use it to turn `H : andb true b2 = true` into `H : b2 = true`. *)
+    split. (* conjunctions can be introduced using the `split` tactic *)
+    + reflexivity.
+    + assumption. (* This goal precisely matches a hypothesis, so we can use the
+      `assumption` tactic. *)
+  - (* case `b1 = false` *)
+    (* Like in the first case, we proceed by simplifying `H`. *)
+    simpl in H.
+    (* This yields `false = true`, which is contradictory. We can now thus use
+    the `discriminate` tactic to discharge the goal. *)
+    discriminate.
+Qed.
+
+(*
+Let us take a look at another example, for which we will define the XOR
+operation on Booleans, which is true iff exactly one of the arguments is true.
+*)
+Definition xorb (b1 b2 : bool) :  bool :=
+  match b1, b2 with
+  | true, false => true
+  | false, true => true
+  | _, _ => false
+  end.
+
+Lemma xorb_inj_l : forall b1 b2 b3 : bool,
+  xorb b1 b2 = xorb b1 b3 -> b2 = b3.
+Proof.
+  intros b1 b2 b3 H.
+  (* Since xor is defined by pattern matching on both arguments, we proceed
+  by making a case distinction on all Boolean variables. *)
+  destruct b1, b2, b3; simpl in H.
+  (* This gives `2^3 = 8`, but as we can see, these can be classified into
+  two kinds:
+  - Trivial goals: `true = true` and `false = false`.
+  - Contradictory goals, where we have either the hypothesis `false = true` or
+    `true = false`.
+  Of course, we could prove each of these goals individually, but that gets
+  pretty boring. So, instead we will make use of of another tactic combinator:
+
+    tac1 || tac2
+
+  This operator will try to run the tactic `tac1` and in case it fails, it will
+  run `tac2` instead.
+  *)
+
+Restart. (* Let us start over *)
+
+  intros b1 b2 b3 H.
+  destruct b1, b2, b3; simpl in H; discriminate || reflexivity.
+Qed.
+
+(* ### Exercises *)
+(* Prove the following lemmas. Note that one can "cheat" by finishing proofs
+with the `Admitted` command. We do this for exercises, and the idea is that
+you finish the proofs. *)
+Lemma xorb_diag_is_true : forall b : bool, xorb b b = b -> b = false.
+Proof. Admitted.
+
+Lemma orb_false_inv : forall b1 b2 : bool,
+  orb b1 b2 = false -> b1 = false /\ b2 = false.
+Proof. Admitted.
+
+Lemma xorb_comm : forall b1 b2, xorb b1 b2 = xorb b2 b1.
+Proof. Admitted.
+
+Lemma xorb_assoc : forall b1 b2 b3 : bool,
+  xorb b1 (xorb b2 b3) = xorb (xorb b1 b2) b3.
+Proof. Admitted.
+
+Lemma xorb_true_inv : forall b1 b2 : bool,
+  xorb b1 b2 = true -> b1 <> b2.
+Proof. Admitted.
+
+Lemma xorb_false_inv : forall b1 b2 : bool,
+  xorb b1 b2 = false -> b1 = b2.
+Proof. Admitted.
+
+(* ## Natural numbers *)
+Module nat_defs.
+(*
+Another very commonly used data type is the natural numbers 0, 1, 2, 3, ... Ome
+can define the natural numbers `nat` in Coq as the Peano numerals:
+*)
+Inductive nat : Type :=
+  | O : nat
+  | S : nat -> nat.
+
+(*
+The type `nat` has two constructors, `O`, which represents the natural number
+`0`, and the constructor `S n`, which represents the natural number `n + 1`.
+Using this data type, we can construct any natural number, for example:
+
+  1 = S O
+  2 = S (S O)
+  3 = S (S (S O))
+  4 = S (S (S (S O)))
+
+And so on. What is different from the type `bool` of Booleans, that we have just
+seen, is that the `nat` is _recursive_: the constructor `S` has an argument of
+type `nat`.
+
+An important feature of recursive inductive types in Coq is that we can define
+functions by structural recursion, for example:
+*)
+
+Fixpoint plus (n1 n2 : nat) : nat :=
+  match n1 with
+  | O => n2
+  | S n1' => S (plus n1' n2)
+  end.
+
+(*
+The above function implements addition of Peano natural numbers, simply by
+merging together the `S` constructors.
+
+It is important to note that the function is structurally recursive on the
+argument `n1`, i.e. the size of the argument `n1` reduces in each recursive
+call. For reasons of soundness of the logic, all functions in Coq should be
+total. Since it is undecidable to check whether a function is total, Coq imposes
+this restriction by requiring each recursive function to be structurally
+recursive. The following definitions are thus not allowed:
+*)
+
+Fail Fixpoint foo (n : nat) := S (foo n).
+Fail Fixpoint bar (n : nat) := S (bar (S n)).
+
+(*
+Both of these attempts result in the error:
+
+  Recursive call to foo has principal argument equal to "n" instead of
+  a sub-term of "n".
+
+Indeed, this function would not terminate, try to simplify `foo 0`, for example.
+
+In similar style as we have defined addition, we can define multiplication. Note
+that this function is structurally recursive in its first argument, and thus Coq
+allows it. *)
+Fixpoint mult (n1 n2 : nat) : nat :=
+  match n1 with
+  | O => O
+  | S n1' => plus n2 (mult n1' n2)
+  end.
+End nat_defs.
+
+(*
+Now that we have defined some operations on natural numbers, let us try to see
+whether we can prove some properties about them.
+
+Note that since we closed the module `nat_defs` above, its content is hidden,
+which allows us to use the natural numbers from Coq's instead. For these we have
+the usual notations, like `0`, `1`, `2`, and so on for the literals, and `+`
+and `*` for the addition and multiplication.
+*)
+
+Lemma plus_0_l : forall n : nat, 0 + n = n.
+Proof.
+  intros n.
+  simpl.
+  reflexivity.
+Qed.
+
+(*
+This proof was simple: since `plus` is defined by recursion on the first
+argument, we can just prove the lemma by computation. Now let us try the version
+with 0 for the second argument.
+*)
+
+Lemma plus_0_r : forall n : nat, n + 0 = n.
+Proof.
+  intros n.
+  simpl. (* Does not do anything, there is no constructor in match position *)
+
+  (* We could try to proceed by case distinction on n, which is done using
+  the destruct tactic. The syntax `as [|n']` is used to name the argument of
+  the constructor `S`. *)
+  destruct n as [|n'].
+  - simpl. reflexivity. (* So good so far. *)
+  - simpl. (* Now we end up with `S (n' + 0) = S n'`, which did not make the
+    situation much better. We quite clearly need something more here... *)
+
+Restart.
+  intros n.
+
+  (* Perform proof by induction. *)
+  induction n as [|n' IH].
+  - simpl. reflexivity.
+  - simpl.
+    rewrite IH. (* replaces the LHS of `IH : n' + 0 = n` with the RHS. *)
+
+    (* Now we have the same goal as before, but with the additional hypothesis
+
+      IH : n' + 0 = n'
+
+    That is to say, we now that the property holds for the smaller natural
+    number `n'`. Thus gives us enough information to finish the proof. *)
+    reflexivity.
+Qed.
+
+(*
+In summary, in the above we have seen two new techniques:
+
+- _Proof by induction_ : using the tactic `induction n as [|n IH]` we can
+  perform induction on a natural number `n`. It will produce two subgoals, one
+  for the base case, and one for the inductive case. The induction hypothesis
+  will be called `IH`.
+- _Proof by rewriting_ : using the tactic `rewrite H` we can substitute an
+  equality `H : x = y` into the goal.
+*)
+
+Lemma plus_S_r : forall n1 n2, n1 + S n2 = S (n1 + n2).
+Proof.
+  intros n1 n2.
+  induction n1 as [|n1 IH].
+  - simpl. reflexivity.
+  - simpl. rewrite IH. reflexivity.
+
+Restart.
+
+(*
+Instead of `rewrite`, we will now demonstrate another tactic: `f_equal`, which
+makes use of the fact that `p = q` implies `S p = S q`.
+*)
+
+  intros n1 n2.
+  induction n1 as [|n1 IH].
+  - simpl. reflexivity.
+  - simpl.
+    f_equal.
+    assumption.
+Qed.
+
+(*
+Think carefully on which argument we should do induction.
+*)
+Lemma plus_assoc : forall n1 n2 n3 : nat,
+  n1 + (n2 + n3) = (n1 + n2) + n3.
+Proof.
+  intros n1 n2 n3.
+  induction n1 as [|n1 IH].
+  - simpl. reflexivity.
+  - simpl. f_equal. assumption.
+Qed.
+
+(*
+In the below, we will see that we can reuse lemmas that we have proved before.
+This is important, as otherwise proofs become quickly unmanageable.
+*)
+Lemma plus_comm : forall n1 n2 : nat, n1 + n2 = n2 + n1.
+Proof.
+  intros n1 n2.
+  induction n1 as [|n1 IH].
+  - simpl.
+    rewrite plus_0_r. (* The goal `n2 = n2 + 0` is an instance of the lemma
+    `plus_0_r` that we proved before. We can use the `rewrite` tactic not just
+    with hypotheses, but also with lemmas. *)
+    reflexivity.
+  - simpl.
+    rewrite plus_S_r. (* In this case, we make use of the lemma `plus_S_r` that
+    we just proved. *)
+    rewrite IH. reflexivity.
+Qed.
+
+(*
+Now that we have seen some proofs by induction, the `induction` tactic may seem
+like a good opportunity to prove any lemma. However, that is not always a good
+idea. As the lemma that we consider next will show, reuse of lemmas, instead of
+blindly performing induction, is very important. The lemma below can be proven
+simply by making use of the properties we have proven so far: associativity and
+commutativity of addition.
+*)
+Lemma plus_rearrange : forall n m p q : nat,
+  (n + m) + p + q = (m + n) + (p + q).
+Proof.
+  intros n m p q.
+  (* The situation here becomes a bit tricky: if we would just write
+  `rewrite plus_comm` it will trigger the rewrite at some arbitrary position in
+  the goal. More precisely, since `plus_comm` is university quantified:
+
+    plus_comm : forall n1 n2 : nat, n1 + n2 = n2 + n1
+
+  It fits any occurrence of plus in the goal. To work around that, we first
+  specialize the lemma, and then rewrite. This is done by partially applying the
+  lemma, as shown below. *)
+  rewrite (plus_comm n).
+
+  (* For associativity we have the same problem, so we perform the same trick. *)
+  rewrite (plus_assoc (m + n)).
+
+  reflexivity.
+Qed.
+
+(*
+To convince yourself, you could give it a try to prove the lemma above by
+induction, and you will see that it gets very difficult.
+*)
+
+(*
+In order to practice some more with proof by induction, we will now define the
+function `beq_nat : nat -> nat -> bool` that computes whether two natural
+numbers are equal.
+
+Note that this function is very different from the equality `=`, which is a
+statement in logic/mathematics, and not a computable function. (The type of
+`n1 = n2` is `Prop`, Coq's type of propositions, whereas the type of
+`beq_nat n1 n2` is `bool`. We will prove:
+
+  n1 = n2 <-> beq_nat n1 n2 = true
+*)
+Fixpoint beq_nat (n1 n2 : nat) : bool :=
+  match n1, n2 with
+  | O, O => true
+  | S n1', S n2' => beq_nat n1' n2'
+  | _, _ => false
+  end.
+
+(*
+For proving the left to right direction, we first introduce a helper lemma.
+*)
+Lemma beq_nat_refl : forall n : nat, beq_nat n n = true.
+Proof.
+  intros n.
+  induction n as [|n IH].
+  - simpl. reflexivity.
+  - simpl. assumption.
+Qed.
+
+Lemma eq_beq_nat : forall n1 n2, n1 = n2 -> beq_nat n1 n2 = true.
+Proof.
+  intros n1 n2 H.
+  rewrite H.
+  rewrite beq_nat_refl.
+  reflexivity.
+Qed.
+
+(*
+The right to left direction will be a but more involved, as we will see.
+*)
+Lemma beq_nat_eq : forall n1 n2, beq_nat n1 n2 = true -> n1 = n2.
+Proof.
+  intros n1 n2 H.
+  induction n1 as [|n1 IH].
+  - simpl in H. destruct n2 as [|n2].
+    + reflexivity.
+    + discriminate.
+  - simpl in H. destruct n2 as [|n2].
+    + discriminate.
+    + (* Now we have to prove `S n1 = S n2`, but our induction hypothesis
+
+        IH : beq_nat n1 (S n2) = true -> n1 = S n2
+
+      Does not really help; it is too weak. If we look at the definition of
+      `beq_nat` we see that `n2` also decreases in each recursive call. In our
+      proof, we however fixed `n2` before doing the induction, and to that end,
+      the induction hypothesis is too specific.  *)
+
+Restart.
+
+  intros n1 n2 H.
+  revert n2 H. (* We fix this problem by generalizing over `n2` and `H` before
+  performing the induction. As we will see, that will give a stronger induction
+  hypothesis that applies to any `n2`. Generalization is done using Coq's
+  `revert` tactic. *)
+  induction n1 as [|n1 IH].
+  - intros n2 H.
+    simpl in H. destruct n2 as [|n2].
+    + reflexivity.
+    + discriminate.
+  - intros n2 H.
+    simpl in H. destruct n2 as [|n2].
+    + discriminate.
+    + (* Now we see that the induction hypothesis is:
+
+         IH : forall n2 : nat, beq_nat n1 n2 = true -> n1 = n2
+
+      This suffices to prove the goal. *)
+      f_equal. apply IH. assumption.
+Qed.
+
+(*
+The technique of generalizing the goal before performing induction is called
+_generalizing the induction hypothesis_. It is often needed.
+
+In the following lemma, we demonstrate Coq's `injection` tactic, which
+simplifies a hypothesis using injectivity of constructors. *)
+Lemma plus_inj_l : forall n1 n2 n3 : nat,
+  n1 + n2 = n1 + n3 -> n2 = n3.
+Proof.
+  intros n1 n2 n3 H. induction n1 as [|n1 IH].
+  - simpl in H.
+    assumption.
+  - simpl in H.
+    apply IH.
+    injection H as H. (* The `injection` tactic applies the fact that
+    constructors of inductive data types are injective. For the case of natural
+    numbers that means:
+
+      S p = S q -> p = q
+
+    *)
+    assumption.
+Qed.
+
+(* ### Exercise (easy to moderate) *)
+(*
+Prove the lemmas below.  For each of the lemmas carefully take into account:
+- Can you derive it from results you have proven already?
+- If not, do you have to perform induction? If so, on which variable?
+- Do you need to generalize the induction hypothesis?
+*)
+Lemma mult_0_l : forall n,
+  0 * n = 0.
+Proof. Admitted.
+
+Lemma mult_0_r : forall n,
+  n * 0 = 0.
+Proof. Admitted.
+
+Lemma plus_swap : forall n1 n2 n3 : nat,
+  n1 + (n2 + n3) = n2 + (n1 + n3).
+Proof. Admitted.
+
+Lemma mult_S_r : forall n1 n2 : nat,
+  n1 * S n2 = n1 + n1 * n2.
+Proof. Admitted.
+
+
+Lemma mult_comm : forall n1 n2 : nat,
+  n1 * n2 = n2 * n1.
+Proof. Admitted.
+
+
+Lemma plus_mult_distr_l : forall n1 n2 n3 : nat,
+  (n1 + n2) * n3 = n1 * n3 + n2 * n3.
+Proof. Admitted.
+
+
+Lemma mult_assoc : forall n1 n2 n3 : nat,
+  n1 * (n2 * n3) = (n1 * n2) * n3.
+Proof. Admitted.
+
+Lemma double_inj : forall n m,
+  n + n = m + m ->
+  n = m.
+Proof. Admitted.
+
+Lemma plus_inj_r : forall n1 n2 n3 : nat,
+  n1 + n3 = n2 + n3 -> n1 = n2.
+Proof. Admitted.
+
+(* ### Exercise (easy) *)
+(*
+Recall the mathematical definition of the factorial function:
+
+    factorial(0) = 1
+    factorial(n) = n * factorial(n - 1)     (if n > 0)
+
+Translate this into a corresponding function in Coq.
+*)
+
+(*
+Fixpoint factorial (n : nat) : nat :=
+  ...
+*)
+
+(* ### Exercise (moderate) *)
+(*
+A small island in the middle of the Pacific Ocean has coins of just two values:
+
+- 3 cents
+- 5 cents
+
+It is claimed that using any amount of 8 cents or more can be composed of a
+combination of these 3 cent and 5 cent coins. Prove this.
+
+Hint: in this proof you may use the `omega` tactic, which solves goals involving
+propositional logic, the operations `=` and `+`, and multiplication by constant
+natural numbers.
+*)
+
+Lemma coin_problem : forall x, exists y z, x + 8 = 3 * y + 5 * z.
+Admitted.
+End lecture.
+
+(* # Advanced data structures *)
+(* ## Finite maps *)
+(*
+In the last part of this course we will look into a way of representing finite
+maps (aka finite partial functions) from natural numbers to elements of some
+type `A`. This means that we want to define a type `map A` and the following
+operations:
+
+  mlookup : map A -> nat -> option A
+  mempty : map A
+  msingleton : nat -> A -> map A
+  minsert : nat -> A -> map A -> map A
+  mdelete : nat -> map A -> map A
+
+These operations should enjoy their expected properties, for example:
+
+  mlookup (minsert i y m) i = Some y
+  i <> j -> mlookup (minsert i y m) j = mlookup m j
+
+The naive way of encoding finite maps is by means of association lists, i.e. as
+lists of key value lists. In Coq that would be:
+*)
+
+Definition assoc_list (A : Type) : Type := list (prod nat A).
+
+Print prod.
+(*
+Inductive prod (A B : Type) : Type :=
+  | pair : A -> B -> A * B
+*)
+
+Print list.
+(*
+Inductive list (A : Type) : Type :=
+  | nil : list A
+  | cons : A -> list A -> list A
+*)
+
+(*
+However, this encoding is not ideal, and suffers from some problems. First of
+all, the same finite maps can be represented by different association lists.
+For example, the map `0 |-> a, 3 |-> b` can be represented by the following
+association lists:
+
+  [(0,a); (3,b)]
+  [(3,b); (0,a)]
+
+This situation is not desired, since it means that the following property does
+_not_ hold:
+
+  m1 = m2 <-> forall i, mlookup m1 i = mlookup m2 i
+
+To see that it does not hold, take
+
+  m1 = [(0,a); (3,b)]
+  m2 = [(3,b); (0,a)]
+
+Now it is clear to see that the property does not hold.
+
+Similarly, another issue of the representation through association lists is that
+the same key could appear multiple times in the same association list, e.g.:
+
+  [(0,a); (0,b)]
+
+When implementing `mlookup` we have to make an arbitrary choice with key/value
+pair to pick. Also, other operations get a bit tricky on how to consider
+duplicate key pairs.
+
+So, a natural question comes up:
+
+  Can we represent finite maps in a different way so that these problems
+  fo not occur?
+
+As we will see, the answer is "yes". To get there, let's first take a look at
+another attempt:
+*)
+
+Definition map_raw (A : Type) := list (option A).
+
+Print option.
+(*
+Inductive option (A : Type) : Type :=
+  | Some : A -> option A
+  | None : option A
+*)
+
+(*
+The idea of this representation is that at each index `i` of the list we have
+`Some a` iff `i |-> a` is in the map, and use `None`s for unused positions. For
+example, we represent the map `0 |-> a, 3 |-> b` as
+
+  [Some a; None; None; Some b]
+
+With the above representation of finite maps in hand, we can now define the
+lookup function as:
+*)
+
+Fixpoint mlookup_raw {A} (m : map_raw A) (i : nat) : option A :=
+  match m with
+  | nil => None
+  | x :: m =>
+     match i with
+     | 0 => x
+     | S i => mlookup_raw m i
+     end
+  end.
+
+(*
+This new representation solves the problem of duplicate keys value pairs, simply
+because at each position in the list, there can be at most one value. However,
+this representation still suffers from the problem that there are duplicate
+representations of the same map. For example, the map in the previous example
+could also be represented by:
+
+  [Some a; None; None; Some b; None]
+  [Some a; None; None; Some b; None; None]
+
+So, in order to have the property
+
+  m1 = m2 <-> forall i, mlookup m1 i = mlookup m2 i
+
+We have to make sure that there is no sequence of `None`s at the end of the
+list. We will do this by considering the "subtype of `raw_map`s that do not have
+a sequence of `None`s at the end". But how to represent subtypes in Coq? As
+we will see below, we do this as follows:
+
+1. Define a predicate that carved out the _well-formed_ `raw_map`s, i.e. those
+   that do not have a sequence of `None`s at the end.
+2. Construct the subtype of _well-formed` `raw_map`s.
+
+Before going into details about the second point, we will first define the
+well-formedness predicate. For reasons that will become apparent later, we do
+this by defining a Boolean function `map_wf`:
+*)
+
+Definition is_Some {A} (x : option A) : bool :=
+  match x with
+  | Some _ => true
+  | None => false
+  end.
+
+Fixpoint map_wf {A} (may_be_nil : bool) (m : map_raw A) : bool :=
+  match m with
+  | [] => may_be_nil
+  | x :: m => map_wf (is_Some x) m
+  end.
+
+(*
+We use the parameter `may_be_nil` to keep track of whether the previous element
+was a `Some`. Only if that is the case, the list may be `nil`.
+
+Now, to define our actual `map` type, we want to consider the elements of type
+`map_raw` that are well-formed. We achieve this by defining a dependently typed
+record that consists of:
+
+- The raw map `m : map_raw`
+- A proof that the raw map `m` is well-formed.
+
+The second becomes part is a bit more subtle. We have defined the well-formedness
+predicate as a Boolean function, whereas proofs in Coq as of type `Prop`. To
+make things work, we thus need to turn the Boolean into a `Prop`. We do this by
+defining a function `is_True : bool -> Prop`:
+*)
+
+Coercion is_True (b : bool) : Prop :=
+  if b then True else False.
+
+(*
+The keyword `Coercion` is used to instruct Coq to automatically insert the
+function whenever it sees a `bool` but needs a `Prop`. We can now for example
+write things like:
+*)
+
+Check (true : Prop).
+Check (true /\ 0 = 0).
+
+(*
+When we instruct Coq to display coercions (by setting `Set Printing Coercions`),
+we see that the above terms actually expand to:
+
+  is_True true : Prop
+  is_True true /\ 0 = 0
+
+With the coercion `is_True` in hand, we can now define the dependently typed
+record as follows:
+*)
+
+Record map (A : Type) := make_map {
+  map_car : map_raw A;
+  map_prf : map_wf true map_car
+}.
+
+(*
+Now let is take a look at the record `map` that we have just defined. As part of
+this, we get a constructor:
+
+  make_map : forall (A : Type) (m : map_raw A), map_wf true m -> map A
+
+And two projections to get out the raw map and the proof, respectively:
+
+  map_car : forall (A : Type), map A -> map_raw A
+  map_prf : forall (A : Type) (m : map A), map_wf true (map_car A m)
+
+The following commands make sure that the type argument `A` becomes implicit,
+so that we do not have to write it explicitly all the time.
+*)
+Arguments make_map {_} _ _.
+Arguments map_car {_} _.
+Arguments map_prf {_} _.
+
+(*
+With the projection `map_car` in hands, it is straightforward to lift the
+function `mlookup_raw` to the record `map` of raw maps together with a proof of
+well-formedness: we just project out the raw map:
+*)
+Definition mlookup {A} (m : map A) (i : nat) : option A :=
+  mlookup_raw (map_car m) i.
+
+(*
+Now that we have the type of maps defined, and the basic operation for looking
+up elements in place, we will start by proving the desired property:
+
+  (forall i, mlookup m1 i = mlookup m2 i) -> m1 = m2
+
+We will do this in two stages:
+
+1. Lemma `map_raw_eq`: Prove that for any `m1 m2 : raw_map A` we have
+
+     map_wf b m1 ->
+     map_wf b m2 ->
+     (forall i, mlookup_raw m1 i = mlookup_raw m2 i) ->
+     m1 = m2
+
+2. Lemma `map_eq`: Show that the desired property follows from (1).
+*)
+
+(*
+Stage 1: We prove the property by induction on one of the raw maps, followed by
+a case distinction on the other. We can pick either `m1` or `m2` for the
+induction, because the choice does not really matter by symmetry, after all.
+
+For the base cases, we will first prove the helper lemma `map_wf_nil` as below.
+This lemma states that whenever we have a well-formed raw map, and looking up
+always yields `None`, then the raw map should be nil. This property is proven
+by induction.
+*)
+Lemma map_wf_nil {A} (b : bool) (m : map_raw A) :
+  map_wf b m ->
+  (forall i, mlookup_raw m i = None) ->
+  m = [].
+Proof.
+  revert b. induction m as [|x m2 IH]; intros b Hwf Hlookup; simpl in *.
+  - reflexivity.
+  - assert (m2 = []).
+    { apply (IH (is_Some x)). apply Hwf. intros i. apply (Hlookup (S i)). }
+    subst m2.
+    assert (x = None).
+    { apply (Hlookup 0). }
+    subst x.
+    simpl in *.
+    destruct Hwf.
+Qed.
+
+(*
+We can now prove the actual property for raw maps. Remember to use the above
+helper lemma in the base cases.
+*)
+Lemma map_raw_eq {A} (b : bool) (m1 m2 : map_raw A) :
+  map_wf b m1 ->
+  map_wf b m2 ->
+  (forall i, mlookup_raw m1 i = mlookup_raw m2 i) -> m1 = m2.
+Proof.
+  revert b m2.
+  induction m1 as [|x m1 IH]; intros b m2 Hm1 Hm2 Hlookup.
+  - symmetry. apply (map_wf_nil b).
+    + apply Hm2.
+    + simpl in *. intros i. symmetry. apply Hlookup.
+  - destruct m2 as [|y m2].
+    + apply (map_wf_nil b). assumption. assumption.
+    + assert (x = y).
+      { apply (Hlookup 0). }
+      subst. simpl in *. f_equal.
+      apply (IH (is_Some y)). assumption. assumption.
+      intros i. apply (Hlookup (S i)).
+Qed.
+
+(*
+Stage 2: We will prove the property for maps, that is:
+
+  (forall i, mlookup m1 i = mlookup m2 i) -> m1 = m2
+
+Unfortunately, even while having the helping lemma `map_raw_eq` that we just
+proved at hand, this direction still does not follow immediately. The problem
+is that maps are essentially tuples
+
+  m : raw_map A
+  H : is_True (map_car true m)
+
+Now if we want to establish that two maps `(m1,H1)` and `(m2,H2)` are equal, we
+do not just have to show that the underlying raw maps `m1` and `m2` are equal
+(which we obtain from `map_raw_eq`), but we also have to show that the proofs
+`H1` and `H2` are equal. So, concretely, after using the equality that `m1` and
+`m2` are equal, we have to show that given:
+
+  m1 : map_raw A
+  H1 : is_True (map_car true m1)
+  H2 : is_True (map_car true m1)
+
+We have to show `H1 = H2`. Intuitively, this may sound obvious, but it is not.
+As you will see in the Homotopy Type Theory lectures, the property below, which
+is typically refered to as _proof irrelevance_ does in general not hold:
+
+  forall (P : Prop) (H1 H2 : P), H1 = H2
+
+Fortunately, in our case we are lucky, we are not considering an arbitrary
+proposition `P`, but something of the shape `is_True b`. Due to that, we can
+actually prove this property by making a case analysis on `b`:
+*)
+Lemma is_True_proof_irrel (b : bool) (H1 H2 : is_True b) :
+  H1 = H2.
+Proof.
+  destruct b; simpl in *.
+  - (* Now we `H1, H2 : True`. By a simple case analysis, we can show that
+    each proof of `True` is equal to `I`, the constructor of `True`. By
+    Curry-Howard, think of `True` as the unit type, and indeed, the only
+    constructor of the unit type is `tt`. *)
+    destruct H1. destruct H2. reflexivity.
+  - (* Now we have `H1, H2 : False`. This is a contradiction. *)
+    destruct H1.
+Qed.
+
+(*
+The desired property, but written as a bi-implication so that we also have the
+opposite direction. Note that the opposite direction of is trivial: we rewrite
+the equality and use reflexivity.
+*)
+Lemma map_eq {A} (m1 m2 : map A) :
+  m1 = m2 <-> forall i, mlookup m1 i = mlookup m2 i.
+Proof.
+  split.
+  - intros ->. reflexivity.
+  - unfold mlookup. intros Hlookup.
+    destruct m1 as [m1 H1], m2 as [m2 H2]; simpl in *.
+    assert (m1 = m2).
+    { apply (map_raw_eq true). apply H1. apply H2. apply Hlookup. }
+    subst m2.
+    f_equal. apply is_True_proof_irrel.
+Qed.
+
+(*
+So, the take home message is that when we want to represent subtypes and have
+sensible results for equality we should:
+
+1. Define a Boolean-valued predicate that expresses well-formedness.
+2. Define a dependently typed record that includes a proof of well-formedness.
+
+The use of a Boolean-valued well-formedness predicate is crucial: it ensures that
+any any two proofs of the well-formedness property are equal, as we have proven
+in the lemma `is_True_proof_irrel`. *)
+
+(*
+## Operations on maps
+
+We will now proceed to define all of the map operations, namely:
+
+  mempty : map A
+  msingleton : nat -> A -> map A
+  minsert : nat -> A -> map A -> map A
+  mdelete : nat -> map A -> map A
+
+The definitions of all of these operations proceeds in the following way:
+
+1. Define the operation on raw maps.
+2. Prove that the operation on raw maps preserves well-formedness.
+3. Lift the operation from raw maps to maps.
+4. Prove the desired properties involving `mlookup_raw` on raw maps.
+5. Lift those properties to a version involving `mlookup`.
+*)
+
+(* ## The empty map *)
+
+Definition mempty_raw {A} : map_raw A := nil.
+
+Lemma mempty_raw_wf {A} : map_wf true (@mempty_raw A).
+Proof. simpl. constructor. Qed.
+
+Definition mempty {A} : map A := make_map mempty_raw mempty_raw_wf.
+
+Lemma mempty_raw_lookup {A} (i : nat) : mlookup_raw (@mempty_raw A) i = None.
+Proof. simpl. reflexivity. Qed.
+
+Lemma mempty_lookup {A} (i : nat) : mlookup (@mempty A) i = None.
+Proof. unfold mlookup, mempty, map_car. apply mempty_raw_lookup. Qed.
+
+(* ## The singleton operation *)
+
+Fixpoint msingleton_raw {A} (i : nat) (y : A) : map_raw A :=
+  match i with
+  | 0 => [Some y]
+  | S i => None :: msingleton_raw i y
+  end.
+
+(* ### Exercise *)
+(*
+Prove the properties of `msingleton` below.
+*)
+Lemma msingleton_raw_wf {A} (b : bool) (i : nat) (y : A) :
+  map_wf b (msingleton_raw i y).
+Proof. Admitted.
+
+Definition msingleton {A} (i : nat) (x : A) : map A :=
+  make_map (msingleton_raw i x) (msingleton_raw_wf true i x).
+
+Lemma msingleton_raw_lookup {A} (i : nat) (y : A) :
+  mlookup_raw (msingleton_raw i y) i = Some y.
+Proof. Admitted.
+
+Lemma msingleton_raw_lookup_ne {A} (i j : nat) (y : A) :
+  i <> j -> mlookup_raw (msingleton_raw i y) j = None.
+Proof.
+  revert i. induction j; intros i; destruct i; simpl in *; eauto.
+  intros []; eauto.
+Admitted.
+
+Lemma msingleton_lookup {A} (i : nat) (y : A) :
+  mlookup (msingleton i y) i = Some y.
+Proof.
+  induction i; eauto.
+Admitted.
+
+Lemma msingleton_lookup_ne {A} (i j : nat) (y : A) :
+  i <> j -> mlookup (msingleton i y) j = None.
+Proof. Admitted.
+
+(* ## The insert operation *)
+
+Fixpoint minsert_raw {A} (i : nat) (y : A) (m : map_raw A) {struct m} : map_raw A :=
+  match m with
+  | [] => msingleton_raw i y
+  | x :: m =>
+    match i with
+    | 0 => Some y :: m
+    | S i => x :: minsert_raw i y m
+    end
+  end.
+
+(* ### Exercise *)
+(*
+Prove the properties of `minsert` below.
+*)
+Lemma map_wf_mono {A} (b : bool) (m : map_raw A) : map_wf b m -> map_wf true m.
+Proof.
+  destruct b; eauto.
+  induction m; eauto.
+  simpl. eauto.
+Qed.
+
+Lemma minsert_raw_wf {A} (b : bool) (i : nat) (y : A) (m : map_raw A) :
+  map_wf b m -> map_wf b (minsert_raw i y m).
+Proof.
+  revert m b. induction i; intros m b.
+  - destruct m; simpl.
+    + eauto.
+    + destruct o; simpl; eauto using map_wf_mono.
+  - intros H. destruct m; simpl; eauto using msingleton_raw_wf.
+Qed.
+
+Definition minsert {A} (i : nat) (x : A) (m : map A) : map A :=
+  match m with
+  | make_map m Hm => make_map (minsert_raw i x m) (minsert_raw_wf true i x m Hm)
+  end.
+
+Lemma minsert_raw_lookup {A} (i : nat) (y : A) (m : map_raw A) :
+  mlookup_raw (minsert_raw i y m) i = Some y.
+Proof. Admitted.
+
+Lemma minsert_raw_lookup_ne {A} (i j : nat) (y : A) (m : map_raw A) :
+  i <> j ->
+  mlookup_raw (minsert_raw i y m) j = mlookup_raw m j.
+Proof.
+  revert j i. induction m; destruct i; destruct j; simpl; eauto.
+  - intros. exfalso. eauto.
+  - intros H. apply msingleton_raw_lookup_ne. omega.
+  - intros. exfalso. eauto.
+Qed.
+
+Lemma minsert_lookup {A} (i : nat) (y : A) (m : map A) :
+  mlookup (minsert i y m) i = Some y.
+Proof. Admitted.
+
+Lemma minsert_lookup_ne {A} (i j : nat) (y : A) (m : map A) :
+  i <> j ->
+  mlookup (minsert i y m) j = mlookup m j.
+Proof. Admitted.
+
+(* ## The delete operation *)
+Fixpoint mcons {A} (x : option A) (m : map_raw A) : map_raw A :=
+  match x with
+  | None =>
+     match m with
+     | [] => []
+     | _ => None :: m
+     end
+  | _ => x :: m
+  end.
+
+Fixpoint mdelete_raw {A} (i : nat) (m : map_raw A) {struct m} : map_raw A :=
+  match m with
+  | [] => []
+  | x :: m =>
+    match i with
+    | 0 => mcons None m
+    | S i => mcons x (mdelete_raw i m)
+    end
+  end.
+
+Lemma mcons_lookup_0 {A} (x : option A) (m : map_raw A) :
+  mlookup_raw (mcons x m) 0 = x.
+Proof. destruct x, m; reflexivity. Qed.
+
+Lemma mcons_lookup_S {A} (x : option A) (m : map_raw A) (i : nat) :
+  mlookup_raw (mcons x m) (S i) = mlookup_raw m i.
+Proof. destruct x, m; reflexivity. Qed.
+
+Arguments mcons : simpl never.
+(* The `Arguments`command with the `simpl never` flag makes sure that `simpl`
+does not unfold `mcons`. This will make some proofs easier, as we rather rewrite
+using the lemmas `mcons_lookup_0` and `mcons_lookup_S` to avoid matches to
+appear in the goal. *)
+
+Lemma mcons_wf {A} (b : bool) (x : option A) (m : map_raw A) :
+  map_wf b m -> map_wf b (mcons x m).
+Proof. destruct m, x; simpl; auto. Qed.
+
+(* ### Exercise *)
+(*
+Prove the properties of `mdelete` below.
+*)
+Lemma mdelete_raw_wf {A} (b : bool) (i : nat) (m : map_raw A) :
+  map_wf b m -> map_wf true (mdelete_raw i m).
+Proof.
+  revert i b. induction m; simpl; eauto; intros i b.
+  destruct i; eauto using mcons_wf, map_wf_mono.
+Admitted.
+
+Definition mdelete {A} (i : nat) (m : map A) : map A :=
+  match m with
+  | make_map m Hm => make_map (mdelete_raw i m) (mdelete_raw_wf true i m Hm)
+  end.
+
+Lemma mdelete_raw_lookup {A} (i : nat) (m : map_raw A) :
+  mlookup_raw (mdelete_raw i m) i = None.
+Proof. Admitted.
+
+Lemma mdelete_raw_lookup_ne {A} (i j : nat) (m : map_raw A) :
+  i <> j ->
+  mlookup_raw (mdelete_raw i m) j = mlookup_raw m j.
+Proof.
+  revert i j. induction m; intros i j; destruct i,j; simpl; eauto.
+  - intros H. exfalso. eauto.
+  - intros _. rewrite mcons_lookup_S. reflexivity.
+  - intros _. rewrite mcons_lookup_0. reflexivity.
+  - intros H. rewrite mcons_lookup_S. apply IHm. eauto.
+Admitted.
+
+Lemma mdelete_lookup {A} (i : nat) (m : map A) :
+  mlookup (mdelete i m) i = None.
+Proof. Admitted.
+
+Lemma mdelete_lookup_ne {A} (i j : nat) (m : map A) :
+  i <> j ->
+  mlookup (mdelete i m) j = mlookup m j.
+Proof. Admitted.
